Saved Work

src/dvspec/dafny/commons.dfy
@@ -122,7 +122,12 @@ module Types
     //     {
     //         this.value
     //     }
-    // }     
+    // } 
+
+
+    datatype ConsensuCommand = 
+        | Start(id: Slot)
+        | Stop(id: Slot)          
 
     datatype Optional<T(0)> = Some(v: T) | None
     {
@@ -171,6 +176,10 @@ module Types
                 Some(e)
         } 
     }         
+}
+
+module CommonFunctions{
+    import opened Types
 
     function method getOrDefault<T1,T2>(M:map<T1,T2>, key:T1, default:T2): T2
     {
@@ -178,5 +187,60 @@ module Types
             M[key]
         else
             default
-    }     
+    }      
+
+    function method compute_start_slot_at_epoch(epoch: Epoch): Slot
+    {
+        epoch * SLOTS_PER_EPOCH
+    }   
+
+    datatype DomainTypes = 
+        | DOMAIN_BEACON_ATTESTER
+
+
+    // TDOO: What about the genesis_validator_root parameter?
+    function method {:extern} compute_domain(
+        domain_type: DomainTypes,
+        fork_version: Version
+    ): (domain: Domain)
+
+
+    lemma {:axiom} compute_domain_properties()
+    ensures forall d1, f1, d2, f2 :: compute_domain(d1, f2) == compute_domain(d2, f2) ==>
+        && d1 == d2 
+        && f1 == f2
+
+    function method {:extern} compute_signing_root<T>(
+        data: T,
+        domain: Domain
+    ): Root
+
+    lemma {:axiom} compute_signing_root_properties<T>()
+    ensures forall da1, do1, da2, do2 ::
+        compute_signing_root<T>(da1, do1) == compute_signing_root<T>(da2, do2) ==>
+            && da1 == da2 
+            && do1 == do2
+
+    // TODO: Fix Python code to match the following (Python code uses epoch)
+    function method compute_attestation_signing_root(attestation_data: AttestationData, fork_version: Version): Root
+    {
+        var domain := compute_domain(DOMAIN_BEACON_ATTESTER, fork_version);
+        compute_signing_root(attestation_data, domain)
+    }
+
+    predicate uniqueSeq<T(==)>(s: seq<T>)
+    {
+        forall i, j | 0 <= i < |s| && 0 <= j < |s| :: s[i] == s[j] ==> i == j
+    }
+
+    predicate {:extern} verify_bls_siganture<T>(
+        data: T,
+        signature: BLSSignature,
+        pubkey: BLSPubkey
+    )   
+
+    function method {:extern} hash_tree_root<T>(data: T): Root 
+
+    lemma {:axiom} hash_tree_root_properties<T>()
+    ensures forall d1: T, d2: T :: hash_tree_root(d1) == hash_tree_root(d2) ==> d1 == d2
 }
