src/dvspec/dafny/dvc_spec.dfy
@@ -1,46 +1,20 @@
 include "commons.dfy"
 include "dvc_implementation.dfy"
 
-module DVCNode_Externs_Proofs refines DVCNode_Externs
-{
+
+abstract module DVCNode_Spec {
+    import opened Types 
+    import opened CommonFunctions
+    import opened DVCNode_Implementation`PublicInterface
+    import opened DVCNode_Externs
+
     function {:axiom} bn_get_fork_version(slot: Slot): Version
 
     function {:axiom} bn_get_validator_index(bnState: BNState, state_id: Root, validator_id: BLSPubkey): (vi: Optional<ValidatorIndex>)
     requires state_id in bnState.state_roots_of_imported_blocks
 
     function {:axiom} bn_get_epoch_committees(bnState: BNState, state_id: Root, index: CommitteeIndex): (sv: seq<ValidatorIndex>) 
-    requires state_id in bnState.state_roots_of_imported_blocks
-
-    datatype BNState = BNState(
-        state_roots_of_imported_blocks: set<Root>   
-    )
-
-    function getInitialBN(): BNState
-    {
-        BNState(
-            state_roots_of_imported_blocks := {}
-        )
-    }
-
-    function toBNState(bn: BeaconNode): BNState
-    reads bn
-    {
-        BNState(
-            state_roots_of_imported_blocks := bn.state_roots_of_imported_blocks
-        )
-    }
-
-    class BeaconNode...
-    {
-        method get_fork_version...
-        ensures bn_get_fork_version(s) == v
-
-        method get_validator_index...
-        ensures state_id in this.state_roots_of_imported_blocks ==> bn_get_validator_index(toBNState(this),state_id, validator_id) == vi
-
-        method get_epoch_committees...
-        ensures state_id in this.state_roots_of_imported_blocks ==> bn_get_epoch_committees(toBNState(this), state_id, index) == sv
-    }
+    requires state_id in bnState.state_roots_of_imported_blocks   
 
     function {:axiom} rs_sign_attestation(
         attestation_data: AttestationData, 
@@ -71,14 +45,18 @@ module DVCNode_Externs_Proofs refines DVCNode_Externs
             && rs_sign_attestation(ad1, fv1, sr1, pk1) == rs_sign_attestation(ad2, fv2, sr2, pk2) 
             ==>
             && sr1 == sr2 
-            && pk1 == pk2 
+            && pk1 == pk2      
 
+    datatype BNState = BNState(
+        state_roots_of_imported_blocks: set<Root>   
+    )
 
-    class RemoteSigner...
+    function getInitialBN(): BNState
     {
-        method sign_attestation...
-        ensures rs_sign_attestation(attestation_data, fork_version, signing_root, toRSState(this)) == s
-    }
+        BNState(
+            state_roots_of_imported_blocks := {}
+        )
+    }    
 
     datatype RSState = RSState(
         pubkey: BLSPubkey
@@ -91,56 +69,7 @@ module DVCNode_Externs_Proofs refines DVCNode_Externs
         RSState(
             pubkey := pubkey
         )
-    }
-
-    function toRSState(
-        rs: RemoteSigner
-    ): RSState
-    reads rs 
-    {
-        RSState(
-            pubkey := rs.pubkey
-        )
-    }
-
-}
-
-module DVCNode_Implementation_Proofs refines DVCNode_Implementation
-{
-    import opened DVCNode_Externs = DVCNode_Externs_Proofs
-
-    export PublicInterface...
-        reveals *
-        // provides 
-        //         toDVCNodeState,
-        //         f_resend_attestation_share,
-        //         toDVCNodeStateAndOuputs,
-        //         Outputs,
-        //         getEmptyOuputs,
-        //         f_att_consensus_decided,
-        //         f_serve_attestation_duty,
-        //         f_listen_for_new_imported_blocks,
-        //         f_listen_for_attestation_shares,
-        //         f_next,
-        //         Event
-        // reveals
-        //         DVCNodeState,
-        //         DVCNodeStateAndOuputs
-        // provides
-        //         DVCNode.network,
-        //         DVCNode.att_consensus, 
-        //         DVCNode.bn,
-        //         DVCNode.current_attesation_duty
-    // export reveals *
-    // export 
-    //     provides Types, DVCNode_Implementation_Helpers, DVCNode_Externs
-    //     reveals DVCNode, toDVCNodeState
-    //     provides 
-    //             DVCNode.serve_attestation_duty, 
-    //             DVCNode.att_consensus_decided, 
-    //             DVCNode.listen_for_attestation_duty_shares,
-    //             DVCNode.listen_for_new_imported_blocks,
-    //             DVCNode.resend_attestation_share
+    }  
 
     datatype DVCNodeState = DVCNodeState(
         current_attesation_duty: Optional<AttestationDuty>,
@@ -154,53 +83,13 @@ module DVCNode_Implementation_Proofs refines DVCNode_Implementation
         future_att_consensus_instances_already_decided: set<Slot>,
         bn: BNState,
         rs: RSState
-    )
-
-    function toDVCNodeState(n: DVCNode): DVCNodeState
-    reads n, n.bn, n.rs
-    {
-        DVCNodeState(
-            current_attesation_duty := n.current_attesation_duty,
-            attestation_duties_queue := n.attestation_duties_queue,
-            attestation_slashing_db := n.attestation_slashing_db,
-            attestation_shares_db := n.attestation_shares_db,
-            attestation_share_to_broadcast := n.attestation_share_to_broadcast,
-            construct_signed_attestation_signature := n.construct_signed_attestation_signature,
-            dv_pubkey := n.dv_pubkey,
-            future_att_consensus_instances_already_decided := n.future_att_consensus_instances_already_decided,
-            bn := toBNState(n.bn),
-            rs := toRSState(n.rs)
-        )
-    }
-
-    function seqToSet<T>(s: seq<T>): (r: set<T>)
-    {
-        set e | e in s
-    }
-
-    function seqMinusToSet<T>(s1: seq<T>, s2: seq<T>): set<T>
-    // requires s2 <= s1 
-    // ensures seqMinus(s1, s2) + s2 == s1
-    {
-        set i | |s2| <= i < |s1| :: s1[i]
-    }
-
-    function seqMinusToOptional<T>(s1: seq<T>, s2: seq<T>): Optional<T>
-    requires s2 <= s1 
-    requires |s1| <= |s2| + 1
-    {
-        if s1 == s2 then
-            None 
-        else
-            Some(s1[|s2|])
-    }
+    )    
 
     datatype Outputs = Outputs(
         att_shares_sent: set<AttestationShare>,
-        att_consensus_commands_sent: set<DVCNode_Externs.ConsensuCommand>,
+        att_consensus_commands_sent: set<ConsensuCommand>,
         attestations_submitted: set<Attestation>
-    )
-
+    )    
 
     function getEmptyOuputs(): Outputs
     {
@@ -209,52 +98,12 @@ module DVCNode_Implementation_Proofs refines DVCNode_Implementation
             {},
             {}
         )
-    }
-
-    twostate predicate onlyOneMaxConsensusCommandAndSubmittedAttestation(n: DVCNode)
-    reads n, n.att_consensus, n.bn
-    {
-        && |n.att_consensus.consensus_commands_sent| <= |old(n.att_consensus.consensus_commands_sent)| + 1
-        && |n.bn.attestations_submitted| <= |old(n.bn.attestations_submitted)| + 1
-    }
-
-    twostate function getOutputs(n: DVCNode): (o: Outputs)
-    reads n, n.network, n.att_consensus, n.bn
-    {
-        Outputs(
-            att_shares_sent :=  seqMinusToSet(n.network.att_shares_sent, old(n.network.att_shares_sent)),
-            att_consensus_commands_sent := seqMinusToSet(n.att_consensus.consensus_commands_sent, old(n.att_consensus.consensus_commands_sent)),
-            attestations_submitted := seqMinusToSet(n.bn.attestations_submitted, old(n.bn.attestations_submitted))
-        )
-    }
+    }    
 
     datatype DVCNodeStateAndOuputs = DVCNodeStateAndOuputs(
         state: DVCNodeState,
         outputs: Outputs
     )
-
-    twostate function toDVCNodeStateAndOuputs(n: DVCNode): DVCNodeStateAndOuputs
-    reads n, n.network, n.att_consensus, n.bn, n.rs
-    {
-        DVCNodeStateAndOuputs(
-            state := toDVCNodeState(n),
-            outputs := getOutputs(n)
-        )
-    }
-
-    function f_update_attestation_slashing_db(attestation_slashing_db: AttestationSlashingDB, attestation_data: AttestationData, attestation_duty_pubkey: BLSPubkey): AttestationSlashingDB     
-    {
-        // assert not is_slashable_attestation_data(attestation_slashing_db, attestation_data, pubkey)
-        // TODO: Is the following required given that each co-validator only handles one pubkey?
-        // slashing_db_data = get_slashing_db_data_for_pubkey(attestation_slashing_db, pubkey)
-        var slashing_db_attestation := SlashingDBAttestation(
-                                            source_epoch := attestation_data.source.epoch,
-                                            target_epoch := attestation_data.target.epoch,
-                                            signing_root := hash_tree_root(attestation_data));
-        
-        attestation_slashing_db + {slashing_db_attestation}
-    }   
-
 
     datatype Event = 
     | ServeAttstationDuty(attestation_duty: AttestationDuty)
@@ -355,7 +204,7 @@ module DVCNode_Implementation_Proofs refines DVCNode_Implementation
                         current_attesation_duty := Some(attestation_duty)
             ),
             outputs := getEmptyOuputs().(
-                att_consensus_commands_sent := {Start(attestation_duty.slot)}
+                att_consensus_commands_sent := {ConsensuCommand.Start(attestation_duty.slot)}
             )
         )        
     }      
@@ -366,6 +215,19 @@ module DVCNode_Implementation_Proofs refines DVCNode_Implementation
     {
         seq(index, i => if i + 1 == index then true else false)
     } 
+
+    function f_update_attestation_slashing_db(attestation_slashing_db: AttestationSlashingDB, attestation_data: AttestationData, attestation_duty_pubkey: BLSPubkey): AttestationSlashingDB     
+    {
+        // assert not is_slashable_attestation_data(attestation_slashing_db, attestation_data, pubkey)
+        // TODO: Is the following required given that each co-validator only handles one pubkey?
+        // slashing_db_data = get_slashing_db_data_for_pubkey(attestation_slashing_db, pubkey)
+        var slashing_db_attestation := SlashingDBAttestation(
+                                            source_epoch := attestation_data.source.epoch,
+                                            target_epoch := attestation_data.target.epoch,
+                                            signing_root := hash_tree_root(attestation_data));
+        
+        attestation_slashing_db + {slashing_db_attestation}
+    }      
 
     function f_att_consensus_decided(
         process: DVCNodeState,
@@ -435,79 +297,79 @@ module DVCNode_Implementation_Proofs refines DVCNode_Implementation
             ) 
     }
  
-        function xxx(
-            process: DVCNodeState,
-            block: BeaconBlock,
-            valIndex: Optional<ValidatorIndex>,
-            i: nat
-        ) : (new_att: set<Slot>)
-        requires i <= |block.body.attestations|
-        requires block.body.state_root in process.bn.state_roots_of_imported_blocks
-        {            
-            set a |
-                    && a in block.body.attestations[..i]
-                    && isMyAttestation(a, process, block, valIndex)
-                    // && a.data.slot == process.attestation_duty.slot 
-                    // && a.data.index == process.attestation_duty.committee_index
-                    // && var committee := bn_get_epoch_committees(process.bn, block.body.state_root, a.data.index);
-                    // && valIndex.Some?
-                    // && valIndex.v in committee
-                    // && var i:nat :| i < |committee| && committee[i] == valIndex.v;
-                    // && i < |a.aggregation_bits|
-                    // && a.aggregation_bits[i]
-                    // && (process.current_attesation_duty.isPresent() ==> a.data.slot >= process.current_attesation_duty.safe_get().slot)
-                ::
-                    a.data.slot
-        }    
+    function xxx(
+        process: DVCNodeState,
+        block: BeaconBlock,
+        valIndex: Optional<ValidatorIndex>,
+        i: nat
+    ) : (new_att: set<Slot>)
+    requires i <= |block.body.attestations|
+    requires block.body.state_root in process.bn.state_roots_of_imported_blocks
+    {            
+        set a |
+                && a in block.body.attestations[..i]
+                && isMyAttestation(a, process, block, valIndex)
+                // && a.data.slot == process.attestation_duty.slot 
+                // && a.data.index == process.attestation_duty.committee_index
+                // && var committee := bn_get_epoch_committees(process.bn, block.body.state_root, a.data.index);
+                // && valIndex.Some?
+                // && valIndex.v in committee
+                // && var i:nat :| i < |committee| && committee[i] == valIndex.v;
+                // && i < |a.aggregation_bits|
+                // && a.aggregation_bits[i]
+                // && (process.current_attesation_duty.isPresent() ==> a.data.slot >= process.current_attesation_duty.safe_get().slot)
+            ::
+                a.data.slot
+    }    
 
-        // function xxxa(
-        //     process: DVCNodeState,
-        //     block: BeaconBlock,
-        //     valIndex: Optional<ValidatorIndex>
-        // ) : (new_att: set<Slot>)
-        // requires block.body.state_root in process.bn.state_roots_of_imported_blocks
-        // {            
-        //     set a |
-        //             && a in block.body.attestations
-        //             // && isMyAttestation(a, process, block, valIndex)
-        //             // && a.data.slot == process.attestation_duty.slot 
-        //             // && a.data.index == process.attestation_duty.committee_index
-        //             && var committee := bn_get_epoch_committees(process.bn, block.body.state_root, a.data.index);
-        //             && valIndex.Some?
-        //             && valIndex.v in committee
-        //             && var i:nat :| i < |committee| && committee[i] == valIndex.v;
-        //             && i < |a.aggregation_bits|
-        //             && a.aggregation_bits[i]
-        //             && (process.current_attesation_duty.isPresent() ==> a.data.slot >= process.current_attesation_duty.safe_get().slot)
-        //         ::
-        //             a.data.slot
-        // }  
+    // function xxxa(
+    //     process: DVCNodeState,
+    //     block: BeaconBlock,
+    //     valIndex: Optional<ValidatorIndex>
+    // ) : (new_att: set<Slot>)
+    // requires block.body.state_root in process.bn.state_roots_of_imported_blocks
+    // {            
+    //     set a |
+    //             && a in block.body.attestations
+    //             // && isMyAttestation(a, process, block, valIndex)
+    //             // && a.data.slot == process.attestation_duty.slot 
+    //             // && a.data.index == process.attestation_duty.committee_index
+    //             && var committee := bn_get_epoch_committees(process.bn, block.body.state_root, a.data.index);
+    //             && valIndex.Some?
+    //             && valIndex.v in committee
+    //             && var i:nat :| i < |committee| && committee[i] == valIndex.v;
+    //             && i < |a.aggregation_bits|
+    //             && a.aggregation_bits[i]
+    //             && (process.current_attesation_duty.isPresent() ==> a.data.slot >= process.current_attesation_duty.safe_get().slot)
+    //         ::
+    //             a.data.slot
+    // }  
 
-        // lemma lxxxx(process: DVCNodeState,
-        //     block: BeaconBlock,
-        //     valIndex: Optional<ValidatorIndex>)
-        //     requires block.body.state_root in process.bn.state_roots_of_imported_blocks
-        // ensures xxx(process, block, valIndex, |block.body.attestations|) == xxxa(process, block, valIndex)
-        // {
-        //     assert block.body.attestations[..|block.body.attestations|] == block.body.attestations;
-        // }           
+    // lemma lxxxx(process: DVCNodeState,
+    //     block: BeaconBlock,
+    //     valIndex: Optional<ValidatorIndex>)
+    //     requires block.body.state_root in process.bn.state_roots_of_imported_blocks
+    // ensures xxx(process, block, valIndex, |block.body.attestations|) == xxxa(process, block, valIndex)
+    // {
+    //     assert block.body.attestations[..|block.body.attestations|] == block.body.attestations;
+    // }           
 
-        predicate isMyAttestation(
-            a: Attestation,
-            process: DVCNodeState,
-            block: BeaconBlock,
-            valIndex: Optional<ValidatorIndex>
-        )
-        requires block.body.state_root in process.bn.state_roots_of_imported_blocks
-        {
-                && var committee := bn_get_epoch_committees(process.bn, block.body.state_root, a.data.index);
-                && valIndex.Some?
-                && valIndex.v in committee
-                && var i:nat :| i < |committee| && committee[i] == valIndex.v;
-                && i < |a.aggregation_bits|
-                && a.aggregation_bits[i]
-                && (process.current_attesation_duty.isPresent() ==> a.data.slot >= process.current_attesation_duty.safe_get().slot)            
-        }
+    predicate isMyAttestation(
+        a: Attestation,
+        process: DVCNodeState,
+        block: BeaconBlock,
+        valIndex: Optional<ValidatorIndex>
+    )
+    requires block.body.state_root in process.bn.state_roots_of_imported_blocks
+    {
+            && var committee := bn_get_epoch_committees(process.bn, block.body.state_root, a.data.index);
+            && valIndex.Some?
+            && valIndex.v in committee
+            && var i:nat :| i < |committee| && committee[i] == valIndex.v;
+            && i < |a.aggregation_bits|
+            && a.aggregation_bits[i]
+            && (process.current_attesation_duty.isPresent() ==> a.data.slot >= process.current_attesation_duty.safe_get().slot)            
+    }
 
     function f_listen_for_new_imported_blocks(
         process: DVCNodeState,
@@ -542,7 +404,7 @@ module DVCNode_Implementation_Proofs refines DVCNode_Implementation
             DVCNodeStateAndOuputs(
                 state := r.state,
                 outputs := r.outputs.(
-                    att_consensus_commands_sent := r.outputs.att_consensus_commands_sent + {Stop(process.current_attesation_duty.safe_get().slot)}
+                    att_consensus_commands_sent := r.outputs.att_consensus_commands_sent + {ConsensuCommand.Stop(process.current_attesation_duty.safe_get().slot)}
                 )
             )
         else
@@ -567,277 +429,53 @@ module DVCNode_Implementation_Proofs refines DVCNode_Implementation
                     )
         )
 
-    }    
-
-    class DVCNode...
-    {
-
-        method update_attestation_slashing_db...
-        ensures f_update_attestation_slashing_db(old(toDVCNodeState(this)).attestation_slashing_db, attestation_data, attestation_duty_pubkey) == this.attestation_slashing_db;  
-
-        method serve_attestation_duty...
-        ensures f_serve_attestation_duty(old(toDVCNodeState(this)), attestation_duty) == toDVCNodeStateAndOuputs(this);
-        {
-            ...;
-            assert f_serve_attestation_duty(old(toDVCNodeState(this)), attestation_duty) == toDVCNodeStateAndOuputs(this);
-        }
-
-        method check_for_next_queued_duty...
-        ensures f_check_for_next_queued_duty(old(toDVCNodeState(this))) == toDVCNodeStateAndOuputs(this);
-        {
-            if...
-            {
-                if...
-                {
-                    ...;
-                    assert f_check_for_next_queued_duty(old(toDVCNodeState(this))) == toDVCNodeStateAndOuputs(this);
-                }
-                else
-                {
-                    ...;
-                    assert f_check_for_next_queued_duty(old(toDVCNodeState(this))) == toDVCNodeStateAndOuputs(this);
-                }
-            }
-            else
-            {
-                assert f_check_for_next_queued_duty(old(toDVCNodeState(this))) == toDVCNodeStateAndOuputs(this);
-            }
-
-        }        
-
-        method start_next_duty...
-        ensures f_start_next_duty(old(toDVCNodeState(this)), attestation_duty) == toDVCNodeStateAndOuputs(this);
-        {
-            ...;
-            assert f_start_next_duty(old(toDVCNodeState(this)), attestation_duty) == toDVCNodeStateAndOuputs(this);
-        }
-
-        method att_consensus_decided...
-        ensures old(this.current_attesation_duty).isPresent() ==> f_att_consensus_decided(old(toDVCNodeState(this)), id, decided_attestation_data) == toDVCNodeStateAndOuputs(this);
-        {
-            ...;
-            if old(this.current_attesation_duty).isPresent()
-            {
-                assert f_att_consensus_decided(old(toDVCNodeState(this)), id, decided_attestation_data) == toDVCNodeStateAndOuputs(this);
-            }
-        }
-
-        method listen_for_attestation_shares...
-        ensures f_listen_for_attestation_shares(old(toDVCNodeState(this)), attestation_share) == toDVCNodeStateAndOuputs(this);
-        {
-            ...;
-        }
-
-        lemma lll<T, T2>(s: seq<T>, p: T -> bool, f: T -> T2, i: nat)
-        requires |s| > 0
-        requires i <= |s| - 1;
-        requires !p(s[i])
-        ensures
-            var S := set a | a in s[..i] && p(a) :: f(a);
-            var S2  := set a | a in s[..i+1] && p(a) :: f(a); 
-            S == S2       
-        {
-            
-
-            var S := set a | a in s[..i] && p(a) :: f(a);
-            var S2  := set a | a in s[..i+1] && p(a) :: f(a);
-
-            assert S == S2;
-        }
-
-
-
-        // lemma l2(block: BeaconBlock, old_future_att_consensus_instances_already_decided: set<Slot>, old_process: DVCNodeState)
-        // requires                 
-        // var new_att := future_att_consensus_instances_already_decided - old_future_att_consensus_instances_already_decided; 
-        // block.body.state_root in old(bn.state_roots_of_imported_blocks) ==>
-        //     new_att == xxx(process, block, valIndex, i);  
-        // {                
-
-        //         var a := block.body.attestations[i];
-        //         var committee :- bn.get_epoch_committees(block.body.state_root, a.data.index);
-
-                
-        //         if
-        //         // && a.data.slot == process.attestation_duty.slot 
-        //         // && a.data.index == process.attestation_duty.committee_index
-        //         && valIndex.Some?
-        //         && valIndex.v in committee
-        //         && var i:nat :| i < |committee| && committee[i] == valIndex.v;
-        //         && i < |a.aggregation_bits|
-        //         && a.aggregation_bits[i]
-        //         && (current_attesation_duty.isPresent() ==> a.data.slot >= current_attesation_duty.safe_get().slot)
-        //         {
-        //             future_att_consensus_instances_already_decided := future_att_consensus_instances_already_decided + {a.data.slot};
-        //         }
-        //         else
-        //         {
-        //             assert 
-        //                 var new_att := future_att_consensus_instances_already_decided - old(this.future_att_consensus_instances_already_decided); 
-        //                 var process := old(toDVCNodeState(this));
-        //                 block.body.state_root in old(bn.state_roots_of_imported_blocks) ==>
-        //                     new_att == xxx(process, block, valIndex, i);   
-
-        //             assert 
-        //                 var new_att := future_att_consensus_instances_already_decided - old(this.future_att_consensus_instances_already_decided); 
-        //                 var process := old(toDVCNodeState(this));
-        //                 block.body.state_root in old(bn.state_roots_of_imported_blocks) ==>
-        //                     new_att == xxx(process, block, valIndex, i + 1);                                                   
-        //         }            
-        // }
-
-        method listen_for_new_imported_blocks...
-        ensures block.body.state_root in bn.state_roots_of_imported_blocks ==> f_listen_for_new_imported_blocks(old(toDVCNodeState(this)), block) == toDVCNodeStateAndOuputs(this);
-        {
-            ...;
-            while...
-                invariant 0 <= i <= |block.body.attestations|
-                invariant  block.body.state_root in old(bn.state_roots_of_imported_blocks) ==>
-                    future_att_consensus_instances_already_decided == 
-                    old(future_att_consensus_instances_already_decided) + xxx(old(toDVCNodeState(this)), block, valIndex, i); 
-                    
-                invariant toDVCNodeState(this) == old(toDVCNodeState(this)).(
-                    future_att_consensus_instances_already_decided := toDVCNodeState(this).future_att_consensus_instances_already_decided
-                )
-                invariant toDVCNodeStateAndOuputs(this).outputs == getEmptyOuputs();            
-            {
-
-            }
-        }
-
-        // method listen_for_new_imported_blocks...
-        // ensures block.body.state_root in bn.state_roots_of_imported_blocks ==> f_listen_for_new_imported_blocks(old(toDVCNodeState(this)), block) == toDVCNodeStateAndOuputs(this);
-        // {
-        //     var valIndex :- bn.get_validator_index(block.body.state_root, dv_pubkey);
-        //     var i := 0;
-
-        //     while i < |block.body.attestations|
-        //         invariant 0 <= i <= |block.body.attestations|
-        //         invariant 
-        //                         var new_att := future_att_consensus_instances_already_decided - old(this.future_att_consensus_instances_already_decided); 
-        //         block.body.state_root in old(bn.state_roots_of_imported_blocks) ==>
-        //             future_att_consensus_instances_already_decided == old(future_att_consensus_instances_already_decided) + xxx(old(toDVCNodeState(this)), block, valIndex, i); 
-
-        //         invariant current_attesation_duty == old(toDVCNodeState(this)).current_attesation_duty;
-        //         invariant toDVCNodeState(this) == old(toDVCNodeState(this)).(
-        //             future_att_consensus_instances_already_decided := toDVCNodeState(this).future_att_consensus_instances_already_decided
-        //         )
-        //         invariant toDVCNodeStateAndOuputs(this).outputs == getEmptyOuputs();
-        //     {
-        //         var a := block.body.attestations[i];
-        //         var committee :- bn.get_epoch_committees(block.body.state_root, a.data.index);
-                                 
-        //         if
-        //         // && a.data.slot == process.attestation_duty.slot 
-        //         // && a.data.index == process.attestation_duty.committee_index
-        //         && valIndex.Some?
-        //         && valIndex.v in committee
-        //         && var i:nat :| i < |committee| && committee[i] == valIndex.v;
-        //         && i < |a.aggregation_bits|
-        //         && a.aggregation_bits[i]
-        //         && (current_attesation_duty.isPresent() ==> a.data.slot >= current_attesation_duty.safe_get().slot)
-        //         {
-        //             future_att_consensus_instances_already_decided := future_att_consensus_instances_already_decided + {a.data.slot};                     
-        //         }
-
-        //         i := i + 1;
-        //     }                           
-
-        //     if current_attesation_duty.isPresent() && current_attesation_duty.safe_get().slot in future_att_consensus_instances_already_decided
-        //     {
-        //         att_consensus.stop(current_attesation_duty.safe_get().slot);
-        //         check_for_next_queued_duty();
-        //     } 
-
-        //     assert block.body.state_root in bn.state_roots_of_imported_blocks ==> f_listen_for_new_imported_blocks(old(toDVCNodeState(this)), block) == toDVCNodeStateAndOuputs(this);
-        // }        
-
-        // method listen_for_new_imported_blocks...
-        // // ensures block.body.state_root in bn.state_roots_of_imported_blocks ==> f_listen_for_new_imported_blocks(old(toDVCNodeState(this)), block) == toDVCNodeStateAndOuputs(this);
-        // {
-        //     ...;
-
-        //     while...
-        //         invariant 0 <= i <= |block.body.attestations|
-        //         // invariant 
-        //         // var new_att := future_att_consensus_instances_already_decided - old(this.future_att_consensus_instances_already_decided); 
-        //         // var process := old(toDVCNodeState(this));
-        //         // block.body.state_root in old(bn.state_roots_of_imported_blocks) ==>
-        //         //     new_att == 
-        //         //         set a |
-        //         //             && a in block.body.attestations[..i]
-        //         //             // && a.data.slot == process.attestation_duty.slot 
-        //         //             // && a.data.index == process.attestation_duty.committee_index
-        //         //             && var committee := bn_get_epoch_committees(process.bn, block.body.state_root, a.data.index);
-        //         //             && valIndex.Some?
-        //         //             && valIndex.v in committee
-        //         //             && var i:nat :| i < |committee| && committee[i] == valIndex.v;
-        //         //             && i < |a.aggregation_bits|
-        //         //             && a.aggregation_bits[i]
-        //         //             && (process.current_attesation_duty.isPresent() ==> a.data.slot >= process.current_attesation_duty.safe_get().slot)
-        //         //          ::
-        //         //             a.data.slot;
-        //     {
-        //         assume                 
-        //         var new_att := future_att_consensus_instances_already_decided - old(this.future_att_consensus_instances_already_decided); 
-        //         var process := old(toDVCNodeState(this));
-        //         block.body.state_root in old(bn.state_roots_of_imported_blocks) ==>
-        //             new_att == 
-        //                 set a |
-        //                     && a in block.body.attestations[..i]
-        //                     // && a.data.slot == process.attestation_duty.slot 
-        //                     // && a.data.index == process.attestation_duty.committee_index
-        //                     && var committee := bn_get_epoch_committees(process.bn, block.body.state_root, a.data.index);
-        //                     && valIndex.Some?
-        //                     && valIndex.v in committee
-        //                     && var i:nat :| i < |committee| && committee[i] == valIndex.v;
-        //                     && i < |a.aggregation_bits|
-        //                     && a.aggregation_bits[i]
-        //                     && (process.current_attesation_duty.isPresent() ==> a.data.slot >= process.current_attesation_duty.safe_get().slot)
-        //                  ::
-        //                     a.data.slot;                
-        //         ...;
-
-        //         if...
-        //         {
-
-        //             assert                 
-        //             var new_att := future_att_consensus_instances_already_decided - old(this.future_att_consensus_instances_already_decided); 
-        //             var process := old(toDVCNodeState(this));
-        //             block.body.state_root in old(bn.state_roots_of_imported_blocks) ==>
-        //                 new_att == 
-        //                     set a |
-        //                         && a in block.body.attestations[..i]
-        //                         // && a.data.slot == process.attestation_duty.slot 
-        //                         // && a.data.index == process.attestation_duty.committee_index
-        //                         && var committee := bn_get_epoch_committees(process.bn, block.body.state_root, a.data.index);
-        //                         && valIndex.Some?
-        //                         && valIndex.v in committee
-        //                         && var i:nat :| i < |committee| && committee[i] == valIndex.v;
-        //                         && i < |a.aggregation_bits|
-        //                         && a.aggregation_bits[i]
-        //                         && (process.current_attesation_duty.isPresent() ==> a.data.slot >= process.current_attesation_duty.safe_get().slot)
-        //                     ::
-        //                         a.data.slot;                    
-        //             ...;
-        //         }
-        //         else
-        //         {
-  
-        //         }
-        //         ...;
-        //     }
-        //     ...;
-        // }
-
-        method resend_attestation_share...
-        ensures f_resend_attestation_share(old(toDVCNodeState(this))) == toDVCNodeStateAndOuputs(this)
-        {
-            ...;
-            assert  f_resend_attestation_share(old(toDVCNodeState(this))) == toDVCNodeStateAndOuputs(this);
-        }
-    }
+    }        
 }
+
+abstract module DVCNode_Externs_Proofs refines DVCNode_Externs
+{
+    import opened DVCNode_Spec
+
+    function toBNState(bn: BeaconNode): BNState
+    reads bn
+    {
+        BNState(
+            state_roots_of_imported_blocks := bn.state_roots_of_imported_blocks
+        )
+    }
+
+    class BeaconNode...
+    {
+        method get_fork_version...
+        ensures bn_get_fork_version(s) == v
+
+        method get_validator_index...
+        ensures state_id in this.state_roots_of_imported_blocks ==> bn_get_validator_index(toBNState(this),state_id, validator_id) == vi
+
+        method get_epoch_committees...
+        ensures state_id in this.state_roots_of_imported_blocks ==> bn_get_epoch_committees(toBNState(this), state_id, index) == sv
+    }
+
+
+    class RemoteSigner...
+    {
+        method sign_attestation...
+        ensures rs_sign_attestation(attestation_data, fork_version, signing_root, toRSState(this)) == s
+    }
+
+    function toRSState(
+        rs: RemoteSigner
+    ): RSState
+    reads rs 
+    {
+        RSState(
+            pubkey := rs.pubkey
+        )
+    }
+
+}
+
+
 
 
 // module A {
