src/dvspec/dafny/dvc_implementation_spec_proof.dfy
@@ -1,0 +1,387 @@
+include "commons.dfy"
+include "dvc_spec.dfy"
+
+abstract module DVCNode_Implementation_Proofs refines DVCNode_Implementation
+{
+    import opened DVCNode_Spec
+    import opened DVCNode_Externs = DVCNode_Externs_Proofs
+
+    export PublicInterface...
+        reveals *
+        // provides 
+        //         toDVCNodeState,
+        //         f_resend_attestation_share,
+        //         toDVCNodeStateAndOuputs,
+        //         Outputs,
+        //         getEmptyOuputs,
+        //         f_att_consensus_decided,
+        //         f_serve_attestation_duty,
+        //         f_listen_for_new_imported_blocks,
+        //         f_listen_for_attestation_shares,
+        //         f_next,
+        //         Event
+        // reveals
+        //         DVCNodeState,
+        //         DVCNodeStateAndOuputs
+        // provides
+        //         DVCNode.network,
+        //         DVCNode.att_consensus, 
+        //         DVCNode.bn,
+        //         DVCNode.current_attesation_duty
+    // export reveals *
+    // export 
+    //     provides Types, DVCNode_Implementation_Helpers, DVCNode_Externs
+    //     reveals DVCNode, toDVCNodeState
+    //     provides 
+    //             DVCNode.serve_attestation_duty, 
+    //             DVCNode.att_consensus_decided, 
+    //             DVCNode.listen_for_attestation_duty_shares,
+    //             DVCNode.listen_for_new_imported_blocks,
+    //             DVCNode.resend_attestation_share
+
+    function toDVCNodeState(n: DVCNode): DVCNodeState
+    reads n, n.bn, n.rs
+    {
+        DVCNodeState(
+            current_attesation_duty := n.current_attesation_duty,
+            attestation_duties_queue := n.attestation_duties_queue,
+            attestation_slashing_db := n.attestation_slashing_db,
+            attestation_shares_db := n.attestation_shares_db,
+            attestation_share_to_broadcast := n.attestation_share_to_broadcast,
+            construct_signed_attestation_signature := n.construct_signed_attestation_signature,
+            dv_pubkey := n.dv_pubkey,
+            future_att_consensus_instances_already_decided := n.future_att_consensus_instances_already_decided,
+            bn := toBNState(n.bn),
+            rs := toRSState(n.rs)
+        )
+    }
+
+    function seqToSet<T>(s: seq<T>): (r: set<T>)
+    {
+        set e | e in s
+    }
+
+    function seqMinusToSet<T>(s1: seq<T>, s2: seq<T>): set<T>
+    // requires s2 <= s1 
+    // ensures seqMinus(s1, s2) + s2 == s1
+    {
+        set i | |s2| <= i < |s1| :: s1[i]
+    }
+
+    function seqMinusToOptional<T>(s1: seq<T>, s2: seq<T>): Optional<T>
+    requires s2 <= s1 
+    requires |s1| <= |s2| + 1
+    {
+        if s1 == s2 then
+            None 
+        else
+            Some(s1[|s2|])
+    }
+
+
+
+
+
+
+    twostate predicate onlyOneMaxConsensusCommandAndSubmittedAttestation(n: DVCNode)
+    reads n, n.att_consensus, n.bn
+    {
+        && |n.att_consensus.consensus_commands_sent| <= |old(n.att_consensus.consensus_commands_sent)| + 1
+        && |n.bn.attestations_submitted| <= |old(n.bn.attestations_submitted)| + 1
+    }
+
+    twostate function getOutputs(n: DVCNode): (o: Outputs)
+    reads n, n.network, n.att_consensus, n.bn
+    {
+        Outputs(
+            att_shares_sent :=  seqMinusToSet(n.network.att_shares_sent, old(n.network.att_shares_sent)),
+            att_consensus_commands_sent := seqMinusToSet(n.att_consensus.consensus_commands_sent, old(n.att_consensus.consensus_commands_sent)),
+            attestations_submitted := seqMinusToSet(n.bn.attestations_submitted, old(n.bn.attestations_submitted))
+        )
+    }
+
+    
+
+    twostate function toDVCNodeStateAndOuputs(n: DVCNode): DVCNodeStateAndOuputs
+    reads n, n.network, n.att_consensus, n.bn, n.rs
+    {
+        DVCNodeStateAndOuputs(
+            state := toDVCNodeState(n),
+            outputs := getOutputs(n)
+        )
+    }
+
+ 
+
+
+
+
+    class DVCNode...
+    {
+
+        method update_attestation_slashing_db...
+        ensures f_update_attestation_slashing_db(old(toDVCNodeState(this)).attestation_slashing_db, attestation_data, attestation_duty_pubkey) == this.attestation_slashing_db;  
+
+        method serve_attestation_duty...
+        ensures f_serve_attestation_duty(old(toDVCNodeState(this)), attestation_duty) == toDVCNodeStateAndOuputs(this);
+        {
+            ...;
+            assert f_serve_attestation_duty(old(toDVCNodeState(this)), attestation_duty) == toDVCNodeStateAndOuputs(this);
+        }
+
+        method check_for_next_queued_duty...
+        ensures f_check_for_next_queued_duty(old(toDVCNodeState(this))) == toDVCNodeStateAndOuputs(this);
+        {
+            if...
+            {
+                if...
+                {
+                    ...;
+                    assert f_check_for_next_queued_duty(old(toDVCNodeState(this))) == toDVCNodeStateAndOuputs(this);
+                }
+                else
+                {
+                    ...;
+                    assert f_check_for_next_queued_duty(old(toDVCNodeState(this))) == toDVCNodeStateAndOuputs(this);
+                }
+            }
+            else
+            {
+                assert f_check_for_next_queued_duty(old(toDVCNodeState(this))) == toDVCNodeStateAndOuputs(this);
+            }
+
+        }        
+
+        method start_next_duty...
+        ensures f_start_next_duty(old(toDVCNodeState(this)), attestation_duty) == toDVCNodeStateAndOuputs(this);
+        {
+            ...;
+            assert f_start_next_duty(old(toDVCNodeState(this)), attestation_duty) == toDVCNodeStateAndOuputs(this);
+        }
+
+        method att_consensus_decided...
+        ensures old(this.current_attesation_duty).isPresent() ==> f_att_consensus_decided(old(toDVCNodeState(this)), id, decided_attestation_data) == toDVCNodeStateAndOuputs(this);
+        {
+            ...;
+            if old(this.current_attesation_duty).isPresent()
+            {
+                assert f_att_consensus_decided(old(toDVCNodeState(this)), id, decided_attestation_data) == toDVCNodeStateAndOuputs(this);
+            }
+        }
+
+        method listen_for_attestation_shares...
+        ensures f_listen_for_attestation_shares(old(toDVCNodeState(this)), attestation_share) == toDVCNodeStateAndOuputs(this);
+        {
+            ...;
+        }
+
+        lemma lll<T, T2>(s: seq<T>, p: T -> bool, f: T -> T2, i: nat)
+        requires |s| > 0
+        requires i <= |s| - 1;
+        requires !p(s[i])
+        ensures
+            var S := set a | a in s[..i] && p(a) :: f(a);
+            var S2  := set a | a in s[..i+1] && p(a) :: f(a); 
+            S == S2       
+        {
+            
+
+            var S := set a | a in s[..i] && p(a) :: f(a);
+            var S2  := set a | a in s[..i+1] && p(a) :: f(a);
+
+            assert S == S2;
+        }
+
+
+
+        // lemma l2(block: BeaconBlock, old_future_att_consensus_instances_already_decided: set<Slot>, old_process: DVCNodeState)
+        // requires                 
+        // var new_att := future_att_consensus_instances_already_decided - old_future_att_consensus_instances_already_decided; 
+        // block.body.state_root in old(bn.state_roots_of_imported_blocks) ==>
+        //     new_att == xxx(process, block, valIndex, i);  
+        // {                
+
+        //         var a := block.body.attestations[i];
+        //         var committee :- bn.get_epoch_committees(block.body.state_root, a.data.index);
+
+                
+        //         if
+        //         // && a.data.slot == process.attestation_duty.slot 
+        //         // && a.data.index == process.attestation_duty.committee_index
+        //         && valIndex.Some?
+        //         && valIndex.v in committee
+        //         && var i:nat :| i < |committee| && committee[i] == valIndex.v;
+        //         && i < |a.aggregation_bits|
+        //         && a.aggregation_bits[i]
+        //         && (current_attesation_duty.isPresent() ==> a.data.slot >= current_attesation_duty.safe_get().slot)
+        //         {
+        //             future_att_consensus_instances_already_decided := future_att_consensus_instances_already_decided + {a.data.slot};
+        //         }
+        //         else
+        //         {
+        //             assert 
+        //                 var new_att := future_att_consensus_instances_already_decided - old(this.future_att_consensus_instances_already_decided); 
+        //                 var process := old(toDVCNodeState(this));
+        //                 block.body.state_root in old(bn.state_roots_of_imported_blocks) ==>
+        //                     new_att == xxx(process, block, valIndex, i);   
+
+        //             assert 
+        //                 var new_att := future_att_consensus_instances_already_decided - old(this.future_att_consensus_instances_already_decided); 
+        //                 var process := old(toDVCNodeState(this));
+        //                 block.body.state_root in old(bn.state_roots_of_imported_blocks) ==>
+        //                     new_att == xxx(process, block, valIndex, i + 1);                                                   
+        //         }            
+        // }
+
+        method listen_for_new_imported_blocks...
+        ensures block.body.state_root in bn.state_roots_of_imported_blocks ==> f_listen_for_new_imported_blocks(old(toDVCNodeState(this)), block) == toDVCNodeStateAndOuputs(this);
+        {
+            ...;
+            while...
+                invariant 0 <= i <= |block.body.attestations|
+                invariant  block.body.state_root in old(bn.state_roots_of_imported_blocks) ==>
+                    future_att_consensus_instances_already_decided == 
+                    old(future_att_consensus_instances_already_decided) + xxx(old(toDVCNodeState(this)), block, valIndex, i); 
+                    
+                invariant toDVCNodeState(this) == old(toDVCNodeState(this)).(
+                    future_att_consensus_instances_already_decided := toDVCNodeState(this).future_att_consensus_instances_already_decided
+                )
+                invariant toDVCNodeStateAndOuputs(this).outputs == getEmptyOuputs();            
+            {
+
+            }
+        }
+
+        // method listen_for_new_imported_blocks...
+        // ensures block.body.state_root in bn.state_roots_of_imported_blocks ==> f_listen_for_new_imported_blocks(old(toDVCNodeState(this)), block) == toDVCNodeStateAndOuputs(this);
+        // {
+        //     var valIndex :- bn.get_validator_index(block.body.state_root, dv_pubkey);
+        //     var i := 0;
+
+        //     while i < |block.body.attestations|
+        //         invariant 0 <= i <= |block.body.attestations|
+        //         invariant 
+        //                         var new_att := future_att_consensus_instances_already_decided - old(this.future_att_consensus_instances_already_decided); 
+        //         block.body.state_root in old(bn.state_roots_of_imported_blocks) ==>
+        //             future_att_consensus_instances_already_decided == old(future_att_consensus_instances_already_decided) + xxx(old(toDVCNodeState(this)), block, valIndex, i); 
+
+        //         invariant current_attesation_duty == old(toDVCNodeState(this)).current_attesation_duty;
+        //         invariant toDVCNodeState(this) == old(toDVCNodeState(this)).(
+        //             future_att_consensus_instances_already_decided := toDVCNodeState(this).future_att_consensus_instances_already_decided
+        //         )
+        //         invariant toDVCNodeStateAndOuputs(this).outputs == getEmptyOuputs();
+        //     {
+        //         var a := block.body.attestations[i];
+        //         var committee :- bn.get_epoch_committees(block.body.state_root, a.data.index);
+                                 
+        //         if
+        //         // && a.data.slot == process.attestation_duty.slot 
+        //         // && a.data.index == process.attestation_duty.committee_index
+        //         && valIndex.Some?
+        //         && valIndex.v in committee
+        //         && var i:nat :| i < |committee| && committee[i] == valIndex.v;
+        //         && i < |a.aggregation_bits|
+        //         && a.aggregation_bits[i]
+        //         && (current_attesation_duty.isPresent() ==> a.data.slot >= current_attesation_duty.safe_get().slot)
+        //         {
+        //             future_att_consensus_instances_already_decided := future_att_consensus_instances_already_decided + {a.data.slot};                     
+        //         }
+
+        //         i := i + 1;
+        //     }                           
+
+        //     if current_attesation_duty.isPresent() && current_attesation_duty.safe_get().slot in future_att_consensus_instances_already_decided
+        //     {
+        //         att_consensus.stop(current_attesation_duty.safe_get().slot);
+        //         check_for_next_queued_duty();
+        //     } 
+
+        //     assert block.body.state_root in bn.state_roots_of_imported_blocks ==> f_listen_for_new_imported_blocks(old(toDVCNodeState(this)), block) == toDVCNodeStateAndOuputs(this);
+        // }        
+
+        // method listen_for_new_imported_blocks...
+        // // ensures block.body.state_root in bn.state_roots_of_imported_blocks ==> f_listen_for_new_imported_blocks(old(toDVCNodeState(this)), block) == toDVCNodeStateAndOuputs(this);
+        // {
+        //     ...;
+
+        //     while...
+        //         invariant 0 <= i <= |block.body.attestations|
+        //         // invariant 
+        //         // var new_att := future_att_consensus_instances_already_decided - old(this.future_att_consensus_instances_already_decided); 
+        //         // var process := old(toDVCNodeState(this));
+        //         // block.body.state_root in old(bn.state_roots_of_imported_blocks) ==>
+        //         //     new_att == 
+        //         //         set a |
+        //         //             && a in block.body.attestations[..i]
+        //         //             // && a.data.slot == process.attestation_duty.slot 
+        //         //             // && a.data.index == process.attestation_duty.committee_index
+        //         //             && var committee := bn_get_epoch_committees(process.bn, block.body.state_root, a.data.index);
+        //         //             && valIndex.Some?
+        //         //             && valIndex.v in committee
+        //         //             && var i:nat :| i < |committee| && committee[i] == valIndex.v;
+        //         //             && i < |a.aggregation_bits|
+        //         //             && a.aggregation_bits[i]
+        //         //             && (process.current_attesation_duty.isPresent() ==> a.data.slot >= process.current_attesation_duty.safe_get().slot)
+        //         //          ::
+        //         //             a.data.slot;
+        //     {
+        //         assume                 
+        //         var new_att := future_att_consensus_instances_already_decided - old(this.future_att_consensus_instances_already_decided); 
+        //         var process := old(toDVCNodeState(this));
+        //         block.body.state_root in old(bn.state_roots_of_imported_blocks) ==>
+        //             new_att == 
+        //                 set a |
+        //                     && a in block.body.attestations[..i]
+        //                     // && a.data.slot == process.attestation_duty.slot 
+        //                     // && a.data.index == process.attestation_duty.committee_index
+        //                     && var committee := bn_get_epoch_committees(process.bn, block.body.state_root, a.data.index);
+        //                     && valIndex.Some?
+        //                     && valIndex.v in committee
+        //                     && var i:nat :| i < |committee| && committee[i] == valIndex.v;
+        //                     && i < |a.aggregation_bits|
+        //                     && a.aggregation_bits[i]
+        //                     && (process.current_attesation_duty.isPresent() ==> a.data.slot >= process.current_attesation_duty.safe_get().slot)
+        //                  ::
+        //                     a.data.slot;                
+        //         ...;
+
+        //         if...
+        //         {
+
+        //             assert                 
+        //             var new_att := future_att_consensus_instances_already_decided - old(this.future_att_consensus_instances_already_decided); 
+        //             var process := old(toDVCNodeState(this));
+        //             block.body.state_root in old(bn.state_roots_of_imported_blocks) ==>
+        //                 new_att == 
+        //                     set a |
+        //                         && a in block.body.attestations[..i]
+        //                         // && a.data.slot == process.attestation_duty.slot 
+        //                         // && a.data.index == process.attestation_duty.committee_index
+        //                         && var committee := bn_get_epoch_committees(process.bn, block.body.state_root, a.data.index);
+        //                         && valIndex.Some?
+        //                         && valIndex.v in committee
+        //                         && var i:nat :| i < |committee| && committee[i] == valIndex.v;
+        //                         && i < |a.aggregation_bits|
+        //                         && a.aggregation_bits[i]
+        //                         && (process.current_attesation_duty.isPresent() ==> a.data.slot >= process.current_attesation_duty.safe_get().slot)
+        //                     ::
+        //                         a.data.slot;                    
+        //             ...;
+        //         }
+        //         else
+        //         {
+  
+        //         }
+        //         ...;
+        //     }
+        //     ...;
+        // }
+
+        method resend_attestation_share...
+        ensures f_resend_attestation_share(old(toDVCNodeState(this))) == toDVCNodeStateAndOuputs(this)
+        {
+            ...;
+            assert  f_resend_attestation_share(old(toDVCNodeState(this))) == toDVCNodeStateAndOuputs(this);
+        }
+    }
+}
